\documentclass [11pt, a4wide, twoside]{article}

\usepackage{times}
\usepackage{epsfig}
\usepackage{ifthen}
\usepackage{xspace}
\usepackage{fancyhdr}
\usepackage{moreverb}
\usepackage{amsmath}
\usepackage{amsthm}

% solution switch
\newboolean{showsolution}
\setboolean{showsolution}{true}

\def\ite{\ensuremath{\mathtt{if~}}}
\def\mul{\ensuremath{\mathtt{mult~}}}
\def\zero{\ensuremath{\mathtt{isZero~}}}
\def\pred{\ensuremath{\mathtt{pred~}}}
\def\succ{\ensuremath{\mathtt{succ~}}}
\def\fst{\ensuremath{\mathtt{1st~}}}
\def\snd{\ensuremath{\mathtt{2nd~}}}
\def\pair{\ensuremath{\mathtt{pair~}}}
\def\true{\ensuremath{\mathtt{True~}}}
\def\false{\ensuremath{\mathtt{False~}}}
\def\l{\ensuremath{\lambda~}}

\input{../include}

\begin{document}

% title
\section*{\ifthenelse{\boolean{showsolution}}{Solution }{}\xspace{}Serie 6 - Fixed Points}

% - - - - - - - - - - - - - - - - - - - - - - - - - - - - - - - - - - - - - - - - - - - - - - - - - - - - - - - - - - - - - - - - - - -
\subsection*{Exercise 1}

We represent non-negative integers with the following Lambda expressions:
%
\begin{align*}
	0 & \equiv \lambda f~.~\lambda x~.~x \\
	1 & \equiv \lambda f~.~\lambda x~.~f x \\
	2 & \equiv \lambda f~.~\lambda x~.~f (f x) \\
	& \vdots  \\
	n & \equiv \lambda f~.~\lambda x~.~f^{n}x
\end{align*}
%
Suppose you have defined the function \textbf{if} and the operations \textbf{add}, \textbf{pred} and \textbf{isZero}. Consider the following recursive (and hence not valid) definition for the multiplication:
%
\begin{equation*}
\textbf{times} = \lambda n_{1}~.~\lambda n_{2}~.~\textbf{if} ~(\textbf{isZero}~ n_{1}) ~\textbf{0}~ (\textbf{add}~ n_{2}~
(\textbf{times} ~(\textbf{pred}~ n_{1}) ~n_{2}))
\end{equation*}
%
If we abstract the name \textbf{times}, we get the new expression:
%
\begin{equation*}
\textbf{t} = \lambda f~.~\lambda n_{1}~.~\lambda n_{2}~.~\textbf{if}~ (\textbf{isZero}~ n_{1}) ~\textbf{0}~ (\textbf{add}~ n_{2}~ (f~ (\textbf{pred}~ n_{1})~ n_{2}))
\end{equation*}
%
By the FP theorem we know that \textbf{(Y t)} is a non-recursive equivalent of the above \textbf{times} definition.\\

\noindent The exercise: write down the reduction sequence to demonstrate that
%
\begin{equation*}
(((\textbf{Y t}) ~\textbf{1}) ~\textbf{k}) \rightarrow \textbf{k}.\\
\end{equation*}
%
\solution{\input{solution1}}


% - - - - - - - - - - - - - - - - - - - - - - - - - - - - - - - - - - - - - - - - - - - - - - - - - - - - - - - - - - - - - - - - - - -
\subsection*{Exercise 2}

We can represent lists and list operators with the following Lambda expressions:
%
\begin{align*}
	\textbf{nil} & = \lambda f~.~true\\
	\textbf{null} & = \lambda l~.~l~(\lambda h~.~\lambda t~.~false)\\
	\textbf{cons} & = \lambda h~.~\lambda t~.~\lambda f~.~f h t\\
	\textbf{head} & = \lambda l~.~l~( \lambda h~.~ \lambda t~.~h)\\
	\textbf{tail} & = \lambda l~.~l~( \lambda h~.~ \lambda t~.~t)
\end{align*}
%
Example: the list $[1,2,3]$ is represented by the $\lambda$-expression \textbf{cons} \textbf{1} (\textbf{cons} \textbf{2} (\textbf{cons} \textbf{3 nil})).\pagebreak

\noindent To do:
%
\begin{enumerate}
\item Translate the following definition into a non-recursive form:
	\begin{equation*}
	\textbf{append} = \lambda~ l_{1} ~.~ \lambda~ l_{2} ~.~\textbf{if}~ (\textbf{null}~ l_{1}) ~l_{2} ~(\textbf{cons} ~(\textbf{head} ~l_{1}) ~ (\textbf{append}~ (\textbf{tail} ~ l_{1}) ~ l_{2}))
	\end{equation*}
\item Test your result by appending list $L_2$ to list $L_1$, which are defined below:
	\begin{align*}
	L_{1}  = \textbf{cons}~\textbf{1} ~(\textbf{cons} ~\textbf{2} ~\textbf{nil})~ \text{ and } ~ L_{2} = \textbf{cons}~ \textbf{3} ~\textbf{nil}\\
	\end{align*}
\end{enumerate}
%

\solution{\input{solution2}t}



\end{document}
