\begin{itemize}
\item b = bound, f = free
\begin{verbatim}
    (\ a b . c d a b) a b (\ c d . d c) (\ e f . f) e
         | | | |  | |          | |           |  |
         f f b b  f f          b b           b  f

\ y . (\ x . z(x(\ x . y(z)))) (\ z . y(x(z)))
             | |       | |            | | |
             f b       b f            b f b
\end{verbatim}


\item 

$\lambda$x.xp \\
p \\
------- -------\\
\texttt{($\lambda$ x . xx) ($\lambda$ x . xx) y} \\
\texttt{($\lambda$ x . xx) ($\lambda$ x . xx) y} \\
\texttt{($\lambda$ x . xx) ($\lambda$ x . xx) y} \\
non-terminating \\



\end{itemize}