and $\equiv$ $\lambda$~x y .~x y x \\
	\indent\indent // if the first argument is \texttt{False}, the function should return \texttt{False}, \ie the first argument; \\
	\indent\indent // if the first argument is \texttt{True}, the function should return the second argument\\
or $\equiv$ $\lambda$~x y .~x x y \\
	\indent\indent // if the first argument is \texttt{True}, the function should return \texttt{True}, \ie the first argument; \\
	\indent\indent // if the first argument is \texttt{False}, the function should return the second argument\\

\texttt{True and False = False}\\
\indent\indent ($\lambda$~x y.~x y x)($\lambda$~x y.~x)($\lambda$~x y.~y) = \\
\indent\indent ($\lambda$~x y.~x)($\lambda$~x y.~y)($\lambda$~x y.~x) = \\
\indent\indent ($\lambda$~x y.~y) $\equiv$ \texttt{False} \\

\texttt{True or False = True}\\
\indent\indent ($\lambda$~x y.~x x y)($\lambda$~x y.~x)($\lambda$~x y.~y) = \\
\indent\indent ($\lambda$~x y.~x)($\lambda$~x y.~x)($\lambda$~x y.~y) = \\
\indent\indent ($\lambda$~x y.~x) $\equiv$ \texttt{True} \\