\documentclass [11pt, a4wide, twoside]{article}

\usepackage{times}
\usepackage{epsfig}
\usepackage{ifthen}
\usepackage{xspace}
\usepackage{fancyhdr}
\usepackage{moreverb}
\usepackage{amsmath,amssymb}

% solution switch
\newboolean{showsolution}
\setboolean{showsolution}{true}

\input{../include}

\begin{document}
%=============================================================================
% title
\section*{Serie 5 - Lambda Calculus}
%=============================================================================
\subsection*{Exercise 1}
%=============================================================================

Consider the following $\lambda$-expressions. Indicate which occurrences of
variables are bound and which ones are free in the expressions.
\begin{enumerate}
\item \texttt{($\lambda$ a b .~c d a b) a b ($\lambda$ c d .~d c)($\lambda$ e f .~f) e}

\item \texttt{\{($\lambda$ u v .~$\lambda$ w .~w ($\lambda$ x .~x(u)) (v)) (y)\} ($\lambda$ z .~$\lambda$ y .~z(y))}

\item \texttt{$\lambda$ y .~($\lambda$ x .~z(x($\lambda$ x .~y(z)))) ($\lambda$ z .~y(x(z)))}
\end{enumerate}

\solution{\fontsize{9pt}{11pt}\verbatimtabinput{exercise1.tex}}

%
%=============================================================================
\subsection*{Exercise 2}
%=============================================================================

Define \verb!true!, \verb!false!, \verb!and!, \verb!or!, \verb!not! and \verb!xor! in Lambda Calculus.
\solution{
\begin{align*}
T &= \lambda ~x ~y ~. ~x \\
F &= \lambda ~x ~y ~. ~y \\
\end{align*}
}

%
%=================================================
\subsection*{Exercise 3}
%=================================================

Reduce the following $\lambda$-expressions to their normal form whenever possible. 

\begin{enumerate}
\renewcommand{\theenumi}{\alph{enumi}}

\item \texttt{P $\equiv$ ($\lambda$ x .~x (x y)) I} ~where \texttt{I $\equiv$ $\lambda$ u .~u}
\solution{%
\begin{align*}
P &= (\lambda ~x ~. ~x ~(x~ y))~ I\\
I~ (I~ y) &= (\lambda ~u ~. ~u) ~((\lambda ~u ~. ~u) ~y)) &~[\text{$\beta$-reduction}]\\
&= (\lambda ~u ~. ~u) ~y &~[\text{$\beta$-reduction}]\\
&= y &~[\text{$\beta$-reduction}]
\end{align*}
}

\item \texttt{Y $\equiv$ $\lambda$ f .~Q Q} ~where \texttt{Q $\equiv$ ($\lambda$ x .~f(x x))}
\solution{%
\begin{align*}
Y &= \lambda ~f ~. ~Q ~Q = \lambda ~f ~. ~(\lambda ~x ~. ~f ~(x ~x)) ~Q\\
&= \lambda ~f ~. ~f ~(Q ~Q) \ldots &~[\text{$\beta$-reduction}]\\
&\text{Does not converge. No normal form exists.}
\end{align*}
}

\item \texttt{L $\equiv$ ($\lambda$ x .~x x y) ($\lambda$ x .~x x y)}
\solution{%
\begin{align*}
L &= (\lambda ~x ~. ~x ~x ~y) ~(\lambda ~x~. ~x ~x ~y) &~[\text{$\beta$-reduction}]\\
& (\lambda ~x ~. ~x ~x ~y) ~(\lambda ~x ~. ~x ~x ~y) ~y &~[\text{$\beta$-reduction}]\\
& (\lambda ~x ~. ~x ~x ~y) ~(\lambda ~x ~. ~x ~x ~y) ~y ~y &~[\text{$\beta$-reduction}]\\
& \ldots\\
& \text{No Normal Form exists.}
\end{align*}
}

\item \texttt{($\lambda$ x .~x L) M} ~where \texttt{M $\equiv$ $\lambda$ x .~y} and \texttt{L $\equiv$ ($\lambda$ x .~x x y) ($\lambda$ x .~x x y)}
\solution{%
\begin{align*}
&(\lambda ~x ~. ~x ~L) ~M &~[\text{$\beta$-reduction}]\\
M L &= (\lambda ~x ~. ~y) ~L  &~[\text{$\beta$-reduction}]\\
&= y
\end{align*}
}

\item \texttt{\{\{$\lambda$ u v .~\{$\lambda$ w .~w ($\lambda$ x .~x(u))\} (v)\} (y)\} ($\lambda$ z .~$\lambda$ y .~z(y))}
\solution{%
\begin{align*}
& \{\{\lambda ~u ~v ~.~\{\lambda ~w ~.~w ~(\lambda ~x ~.~x ~u)\} ~v\} ~y\} ~(\lambda ~z ~.~\lambda ~y ~.~z ~y) &~[\text{$\beta$-reduction}]\\
& \{\{\lambda ~u ~v .~v (\lambda ~x ~.~x~u)\} ~y\} ~(\lambda ~z ~.~\lambda ~y ~.~z~y) &~[\text{$\beta$-reduction}]\\
& \{\lambda ~v .~v (\lambda ~x ~.~x~y)\} ~(\lambda ~z ~.~\lambda ~y ~.~z~y) &~[\text{$\beta$-reduction}]\\
& (\lambda ~z ~.~\lambda ~y ~.~z(y)) ~(\lambda ~x ~.~x(y)) &~[\text{$\alpha$-conversion}]\\
& (\lambda ~z ~.~\lambda ~y' ~.~z~y') ~(\lambda ~x ~.~x~y) &~[\text{$\beta$-reduction}]\\
& \lambda ~y' ~.~(\lambda ~x ~.~x~y)~y' &~[\text{$\beta$-reduction}]\\
& \lambda ~y' ~.~y'~y
\end{align*}
}

\end{enumerate}


\end{document}
